move things to circular table

concurrency/disciplined/sharedexclusive-linearatomic/ShardedHashTable.i.dfy
@@ -1,10 +1,8 @@
-include "../../../lib/Lang/NativeTypes.s.dfy"
-include "../../../lib/Base/Option.s.dfy"
 include "../../../lib/Base/sequences.i.dfy"
 include "../common/ConcurrencyModel.s.dfy"
 include "../common/AppSpec.s.dfy"
 include "../common/CountMonoid.i.dfy"
-include "CircularRange.i.dfy"
+include "CircularTable.i.dfy"
 
 module ShardedHashTable refines ShardedStateMachine {
   import opened NativeTypes
@@ -13,6 +11,7 @@ module ShardedHashTable refines ShardedStateMachine {
   import opened Limits
   import opened KeyValueType
   import opened CircularRange
+  import opened CircularTable
 
   import MapIfc
   import Count
@@ -28,28 +27,6 @@ module ShardedHashTable refines ShardedStateMachine {
     | Stub(rid: int, output: MapIfc.Output)
 
   function DummyKey() : Key
-
-  function method hash(key: Key) : Index
-
-  // This is the thing that's stored in the hash table at this row.
-  datatype Entry =
-    | Full(key: Key, value: Value)
-    | Empty
-
-  type Table = seq<Option<Entry>>
-
-  type FixedTable = t: Table
-    | |t| == FixedSize() witness *
-
-  predicate Complete(table: FixedTable)
-  {
-    forall i: Index :: table[i].Some?
-  }
-
-  function unitTable(): Table
-  {
-    seq(FixedSize(), i => None)
-  }
 
   datatype Variables =
       | Variables(table: FixedTable,
@@ -68,7 +45,7 @@ module ShardedHashTable refines ShardedStateMachine {
 
   function unit() : Variables
   {
-    Variables(unitTable(), Count.Variables(0), multiset{}, multiset{})
+    Variables(UnitTable(), Count.Variables(0), multiset{}, multiset{})
   }
 
   function input_ticket(id: int, input: Ifc.Input) : Variables
@@ -149,7 +126,7 @@ module ShardedHashTable refines ShardedStateMachine {
   predicate IsInputResource(in_r: Variables, rid: int, input: Ifc.Input)
   {
     && in_r.Variables?
-    && in_r.table == unitTable()
+    && in_r.table == UnitTable()
     && in_r.insert_capacity.value == 0
     && in_r.tickets == multiset { Ticket(rid, input) }
     && in_r.stubs == multiset { }
@@ -158,34 +135,6 @@ module ShardedHashTable refines ShardedStateMachine {
 //////////////////////////////////////////////////////////////////////////////
 // Transition definitions
 //////////////////////////////////////////////////////////////////////////////
-
-  function PSL(key: Key, i: Index): nat
-  {
-    var h := hash(key);
-    if h <= i then
-      i - h
-    else
-      FixedSize() - h + i
-  }
-
-  function SlotKeyHash(table: FixedTable, i: Index): Index
-    requires table[i].Some? && table[i].value.Full?
-  {
-    hash(table[i].value.key)
-  }
-
-  function SlotPSL(table: FixedTable, i: Index): nat
-    requires table[i].Some? && table[i].value.Full?
-  {
-    PSL(table[i].value.key, i)
-  }
-
-  type EntryPredicate = (Option<Entry>, Index, Key) -> bool
-
-  predicate TrueInRange(table: FixedTable, range: Range, key: Key, p: EntryPredicate)
-  {
-    forall i: Index | range.Contains(i) :: p(table[i], i, key)
-  }
 
   datatype Step =
     | InsertStep(ticket: Ticket, kv: (Key, Value), start: Index, end: Index)
@@ -245,49 +194,6 @@ module ShardedHashTable refines ShardedStateMachine {
     && PSL(entry.value.key, slot_index) < PSL(insert_key, slot_index)
   }
 
-  predicate IsTableRightShift(table: FixedTable, table': FixedTable, inserted: Option<Entry>, start: Index, end: Index)
-  {
-    && (start <= end ==>
-      && (forall i | 0 <= i < start :: table'[i] == table[i])
-      && table'[start] == inserted
-      && (forall i | start < i <= end :: table'[i] == table[i-1])
-      && (forall i | end < i < |table'| :: table'[i] == table[i]))
-    && (start > end ==>
-      && table'[0] == table[ |table| - 1]
-      && (forall i | 0 < i <= end :: table'[i] == table[i-1])
-      && (forall i | end < i < start :: table'[i] == table[i])
-      && table'[start] == inserted
-      && (forall i | start < i < |table'| :: table'[i] == table[i-1]))
-  }
-
-  function TableRightShift(table: FixedTable, inserted: Option<Entry>, start: Index, end: Index) : (table': FixedTable)
-    ensures IsTableRightShift(table, table', inserted, start, end)
-  {
-    if start <= end then
-      table[..start] + [inserted] + table[start..end] + table[end+1..]
-    else
-      var last_index := |table| - 1;
-      [table[last_index]] + table[..end] + table[end+1..start] + [inserted] + table[start..last_index]
-  }
-  
-  lemma RightShiftIndex(table: FixedTable, table': FixedTable, inserted: Option<Entry>, start: Index, end: Index, i: Index)
-    requires IsTableRightShift(table, table', inserted, start, end)
-    ensures Partial(NextIndex(start), NextIndex(end)).Contains(i) ==> table'[i] == table[PrevIndex(i)];
-    ensures Partial(NextIndex(end), start).Contains(i) ==> table'[i] == table[i];
-    ensures i == start ==> table'[i] == inserted;
-  {
-  }
-
-  lemma RightShiftedPSL(table: FixedTable, table': FixedTable, inserted: Option<Entry>, start: Index, end: Index, i: Index)
-    requires IsTableRightShift(table, table', inserted, start, end)
-    requires table'[i].Some? && table'[i].value.Full?
-    requires Partial(NextIndex(start), NextIndex(end)).Contains(i)
-    requires i != hash(table[PrevIndex(i)].value.key)
-    ensures SlotPSL(table', i) == SlotPSL(table, PrevIndex(i)) + 1
-  {
-    assert table'[i] == table[PrevIndex(i)];
-  }
-
   predicate InsertEnable(v: Variables, step: Step)
   {
     && step.InsertStep?
@@ -319,7 +225,6 @@ module ShardedHashTable refines ShardedStateMachine {
       .(tickets := v.tickets - multiset{ticket})
       .(stubs := v.stubs + multiset{Stub(ticket.rid, MapIfc.InsertOutput(true))})
   }
-
 /*
   predicate OverwriteEnable(v: Variables, step: Step)
   {
@@ -390,30 +295,6 @@ module ShardedHashTable refines ShardedStateMachine {
   }
 
 // Remove transition definitions
-
-  predicate IsTableLeftShift(table: FixedTable, table': FixedTable, start: Index, end: Index)
-  {
-    && (start <= end ==>
-      && (forall i | 0 <= i < start :: table'[i] == table[i]) 
-      && (forall i | start <= i < end :: table'[i] == table[i+1]) 
-      && table'[end] == Some(Empty)
-      && (forall i | end < i < |table'| :: table'[i] == table[i]))
-    && (start > end ==>
-      && (forall i | 0 <= i < end :: table'[i] == table[i+1])
-      && table'[end] == Some(Empty)
-      && (forall i | end < i < start :: table'[i] == table[i])
-      && (forall i | start <= i < |table'| - 1 :: table'[i] == table[i+1])
-      && table'[ |table'| - 1 ] == table[0])
-  }
-
-  function TableLeftShift(table: FixedTable, start: Index, end: Index): (table': FixedTable)
-    ensures IsTableLeftShift(table, table', start, end)
-  {
-    if start <= end then
-      table[..start] + table[start+1..end+1] + [Some(Empty)] + table[end+1..]
-    else
-      table[1..end+1] + [Some(Empty)] + table[end+1..start] + table[start+1..] + [table[0]]
-  }
 
   // NOTE dummy_key not being used
   predicate SlotShouldTidy(entry: Option<Entry>, slot_index: Index, dummy_key: Key)
@@ -519,119 +400,6 @@ module ShardedHashTable refines ShardedStateMachine {
 // global-level Invariant proof
 //////////////////////////////////////////////////////////////////////////////
 
-  // Keys are unique, although we don't count entries being removed
-  predicate KeysUnique(table: FixedTable)
-    requires Complete(table)
-  {
-    forall i: Index, j: Index | 
-        && i != j
-        && table[i].value.Full?
-        && table[j].value.Full?
-      :: table[i].value.key != table[j].value.key
-  }
-
-  predicate ValidHashSegment(table: FixedTable, hash: Index, range: Range)
-    requires Complete(table)
-  {
-    // the segement can only be Partial
-    && range.Partial?
-    // // if the segment is Partial, the hash cannot be in the middle 
-    // && (range.Partial? ==>
-    //   !Contains(Partial(NextIndex(range.start), range.end), hash))
-    // all the keys in the segment share the hash
-    && (forall i: Index | range.Contains(i) ::
-        && table[i].value.Full?
-        && SlotKeyHash(table, i) == hash)
-    // and no where else
-    && (forall i: Index | !range.Contains(i) ::
-        (table[i].value.Full? ==> 
-        SlotKeyHash(table, i) != hash))
-  }
-
-  predicate ExistsHashSegment(table: FixedTable, hash: Index)
-  requires Complete(table)
-  {
-    // there exists a segment of slots that has the matching hash (could be empty)
-    exists range: Range :: ValidHashSegment(table, hash, range)
-  }
-
-  predicate ValidHashSegments(table: FixedTable)
-  requires Complete(table)
-  {
-    forall hash: Index :: ExistsHashSegment(table, hash)
-  }
-
-  function GetHashSegment(table: FixedTable, hash: Index): (Range)
-  requires Complete(table)
-  requires ValidHashSegments(table)
-  ensures ValidHashSegment(table, hash, GetHashSegment(table, hash))
-  {
-    assert ExistsHashSegment(table, hash);
-    var range: Range :|
-      ValidHashSegment(table, hash, range);
-    range
-  }
-
-  lemma ValidHashSegmentsImpliesDisjoint(table: FixedTable, h0: Index, h1: Index)
-    requires h0 != h1
-    requires Complete(table)
-    requires ValidHashSegments(table)
-    ensures !GetHashSegment(table, h0).OverlapsWith(GetHashSegment(table, h1))
-  {
-    var range0 := GetHashSegment(table, h0);
-    var range1 := GetHashSegment(table, h1);
-
-    forall i : Index | range0.Contains(i)
-      ensures !range1.Contains(i)
-    {
-      assert table[i].value.Full?;
-      assert SlotKeyHash(table, i) == h0;
-      assert SlotKeyHash(table, i) != h1;
-    }
-
-    forall i : Index | range1.Contains(i)
-      ensures !range0.Contains(i)
-    {
-      assert table[i].value.Full?;
-      assert SlotKeyHash(table, i) == h1;
-      assert SlotKeyHash(table, i) != h0;
-    }
-  }
-
-  // predicate ValidOrdering(table: FixedTable, h0: Index)
-  // requires Complete(table)
-  // requires ValidHashSegments(table)
-  // {
-  //   var h1 := NextIndex(h0);
-  //   var range0 := GetHashSegment(table, h0);
-  //   var range1 := GetHashSegment(table, h1);
-  //   // this part should all be empty (we won't have a none-empty segment in between)
-  //   (forall i : Index | Contains(GetBetween(range0, range1), i) :: table[i].value.Empty?)
-  // }
-
-  predicate ValidPSL(table: FixedTable, i: Index)
-    requires Complete(table)
-  {
-    table[i].value.Full? ==>
-    (
-      var key := table[i].value.key;
-      var h_i := hash(key);
-      forall j: Index :: Partial(h_i, i).Contains(j) ==> 
-      (
-        && table[j].value.Full?
-        && SlotPSL(table, j) >= PSL(key, j)
-      )
-    )
-  }
-
-  predicate InvTable(table: FixedTable)
-  {
-    && Complete(table)
-    && KeysUnique(table)
-    && ValidHashSegments(table)
-    // && (forall h: Index :: ValidOrdering(table, h))
-    && (forall i: Index :: ValidPSL(table, i))
-  }
 
   function EntryQuantity(entry: Option<Entry>): nat
   {
