concurrency/disciplined/sharedexclusive-linearatomic/CircularTable.i.dfy
@@ -1,0 +1,236 @@
+include "../../../lib/Base/Option.s.dfy"
+include "CircularRange.i.dfy"
+
+module CircularTable {
+  import opened Options
+  import opened CircularRange
+  import opened NativeTypes
+  import opened KeyValueType
+  import opened Limits
+
+  function method hash(key: Key) : Index
+
+  // This is the thing that's stored in the hash table at this row.
+  datatype Entry =
+    | Full(key: Key, value: Value)
+    | Empty
+
+  type Table = seq<Option<Entry>>
+
+  type FixedTable = t: Table
+    | |t| == FixedSize() witness *
+    
+  predicate Complete(table: FixedTable)
+  {
+    forall i: Index :: table[i].Some?
+  }
+
+  // Keys are unique, although we don't count entries being removed
+  predicate KeysUnique(table: FixedTable)
+    requires Complete(table)
+  {
+    forall i: Index, j: Index | 
+        && i != j
+        && table[i].value.Full?
+        && table[j].value.Full?
+      :: table[i].value.key != table[j].value.key
+  }
+
+  predicate ValidHashSegment(table: FixedTable, hash: Index, range: Range)
+    requires Complete(table)
+  {
+    // the segement can only be Partial
+    && range.Partial?
+    // // if the segment is Partial, the hash cannot be in the middle 
+    // && (range.Partial? ==>
+    //   !Contains(Partial(NextIndex(range.start), range.end), hash))
+    // all the keys in the segment share the hash
+    && (forall i: Index | range.Contains(i) ::
+        && table[i].value.Full?
+        && SlotKeyHash(table, i) == hash)
+    // and no where else
+    && (forall i: Index | !range.Contains(i) ::
+        (table[i].value.Full? ==> 
+        SlotKeyHash(table, i) != hash))
+  }
+
+  predicate ExistsHashSegment(table: FixedTable, hash: Index)
+    requires Complete(table)
+  {
+    // there exists a segment of slots that has the matching hash (could be empty)
+    exists range: Range :: ValidHashSegment(table, hash, range)
+  }
+
+  function GetHashSegment(table: FixedTable, hash: Index): (r: Range)
+    requires Inv(table)
+    ensures ValidHashSegment(table, hash, r)
+  {
+    assert ExistsHashSegment(table, hash);
+    var range: Range :|
+      ValidHashSegment(table, hash, range);
+    range
+  }
+
+  predicate ValidPSL(table: FixedTable, i: Index)
+    requires Complete(table)
+  {
+    table[i].value.Full? ==>
+    (
+      var key := table[i].value.key;
+      var h_i := hash(key);
+      forall j: Index :: Partial(h_i, i).Contains(j) ==> 
+      (
+        && table[j].value.Full?
+        && SlotPSL(table, j) >= PSL(key, j)
+      )
+    )
+  }
+
+  predicate Inv(table: FixedTable)
+  {
+    && Complete(table)
+    && KeysUnique(table)
+    // && (forall h: Index :: ValidOrdering(table, h))
+    && (forall i: Index ::
+      && ValidPSL(table, i)
+      && ExistsHashSegment(table, i))
+  }
+
+  function UnitTable(): Table
+  {
+    seq(FixedSize(), i => None)
+  }
+
+  function PSL(key: Key, i: Index): nat
+  {
+    var h := hash(key);
+    if h <= i then
+      i - h
+    else
+      FixedSize() - h + i
+  }
+
+  function SlotKeyHash(table: FixedTable, i: Index): Index
+    requires table[i].Some? && table[i].value.Full?
+  {
+    hash(table[i].value.key)
+  }
+
+  function SlotPSL(table: FixedTable, i: Index): nat
+    requires table[i].Some? && table[i].value.Full?
+  {
+    PSL(table[i].value.key, i)
+  }
+
+  type EntryPredicate = (Option<Entry>, Index, Key) -> bool
+
+  predicate TrueInRange(table: FixedTable, range: Range, key: Key, p: EntryPredicate)
+  {
+    forall i: Index | range.Contains(i) :: p(table[i], i, key)
+  }
+
+  predicate IsTableRightShift(table: FixedTable, table': FixedTable, inserted: Option<Entry>, start: Index, end: Index)
+  {
+    && (start <= end ==>
+      && (forall i | 0 <= i < start :: table'[i] == table[i])
+      && table'[start] == inserted
+      && (forall i | start < i <= end :: table'[i] == table[i-1])
+      && (forall i | end < i < |table'| :: table'[i] == table[i]))
+    && (start > end ==>
+      && table'[0] == table[ |table| - 1]
+      && (forall i | 0 < i <= end :: table'[i] == table[i-1])
+      && (forall i | end < i < start :: table'[i] == table[i])
+      && table'[start] == inserted
+      && (forall i | start < i < |table'| :: table'[i] == table[i-1]))
+  }
+
+  function TableRightShift(table: FixedTable, inserted: Option<Entry>, start: Index, end: Index) : (table': FixedTable)
+    ensures IsTableRightShift(table, table', inserted, start, end)
+  {
+    if start <= end then
+      table[..start] + [inserted] + table[start..end] + table[end+1..]
+    else
+      var last_index := |table| - 1;
+      [table[last_index]] + table[..end] + table[end+1..start] + [inserted] + table[start..last_index]
+  }
+  
+  lemma RightShiftIndex(table: FixedTable, table': FixedTable, inserted: Option<Entry>, start: Index, end: Index, i: Index)
+    requires IsTableRightShift(table, table', inserted, start, end)
+    ensures Partial(NextIndex(start), NextIndex(end)).Contains(i) ==> table'[i] == table[PrevIndex(i)];
+    ensures Partial(NextIndex(end), start).Contains(i) ==> table'[i] == table[i];
+    ensures i == start ==> table'[i] == inserted;
+  {
+  }
+
+  lemma RightShiftedPSL(table: FixedTable, table': FixedTable, inserted: Option<Entry>, start: Index, end: Index, i: Index)
+    requires IsTableRightShift(table, table', inserted, start, end)
+    requires table'[i].Some? && table'[i].value.Full?
+    requires Partial(NextIndex(start), NextIndex(end)).Contains(i)
+    requires i != hash(table[PrevIndex(i)].value.key)
+    ensures SlotPSL(table', i) == SlotPSL(table, PrevIndex(i)) + 1
+  {
+    assert table'[i] == table[PrevIndex(i)];
+  }
+
+  predicate IsTableLeftShift(table: FixedTable, table': FixedTable, start: Index, end: Index)
+  {
+    && (start <= end ==>
+      && (forall i | 0 <= i < start :: table'[i] == table[i]) 
+      && (forall i | start <= i < end :: table'[i] == table[i+1]) 
+      && table'[end] == Some(Empty)
+      && (forall i | end < i < |table'| :: table'[i] == table[i]))
+    && (start > end ==>
+      && (forall i | 0 <= i < end :: table'[i] == table[i+1])
+      && table'[end] == Some(Empty)
+      && (forall i | end < i < start :: table'[i] == table[i])
+      && (forall i | start <= i < |table'| - 1 :: table'[i] == table[i+1])
+      && table'[ |table'| - 1 ] == table[0])
+  }
+
+  function TableLeftShift(table: FixedTable, start: Index, end: Index): (table': FixedTable)
+    ensures IsTableLeftShift(table, table', start, end)
+  {
+    if start <= end then
+      table[..start] + table[start+1..end+1] + [Some(Empty)] + table[end+1..]
+    else
+      table[1..end+1] + [Some(Empty)] + table[end+1..start] + table[start+1..] + [table[0]]
+  }
+
+  // lemma ValidHashSegmentsImpliesDisjoint(table: FixedTable, h0: Index, h1: Index)
+  //   requires h0 != h1
+  //   requires Complete(table)
+  //   requires ValidHashSegments(table)
+  //   ensures !GetHashSegment(table, h0).OverlapsWith(GetHashSegment(table, h1))
+  // {
+  //   var range0 := GetHashSegment(table, h0);
+  //   var range1 := GetHashSegment(table, h1);
+
+  //   forall i : Index | range0.Contains(i)
+  //     ensures !range1.Contains(i)
+  //   {
+  //     assert table[i].value.Full?;
+  //     assert SlotKeyHash(table, i) == h0;
+  //     assert SlotKeyHash(table, i) != h1;
+  //   }
+
+  //   forall i : Index | range1.Contains(i)
+  //     ensures !range0.Contains(i)
+  //   {
+  //     assert table[i].value.Full?;
+  //     assert SlotKeyHash(table, i) == h1;
+  //     assert SlotKeyHash(table, i) != h0;
+  //   }
+  // }
+
+  // predicate ValidOrdering(table: FixedTable, h0: Index)
+  // requires Complete(table)
+  // requires ValidHashSegments(table)
+  // {
+  //   var h1 := NextIndex(h0);
+  //   var range0 := GetHashSegment(table, h0);
+  //   var range1 := GetHashSegment(table, h1);
+  //   // this part should all be empty (we won't have a none-empty segment in between)
+  //   (forall i : Index | Contains(GetBetween(range0, range1), i) :: table[i].value.Empty?)
+  // }
+
+}
